QAL/AbstractStore.v
@@ -1,0 +1,14 @@
+Require Import FSetInterface.
+Require Import Tactics Algebra.Utils SetoidUtils Algebra.SetoidCat  Algebra.Monad Algebra.SetoidCat.PairUtils Algebra.SetoidCat.MaybeUtils Algebra.Monad.Maybe Algebra.Alternative Algebra.Functor Algebra.FoldableFunctor Algebra.Applicative Algebra.Monoid Algebra.SetoidCat.NatUtils Algebra.SetoidCat.BoolUtils Algebra.Monoid.PropUtils QAL.Definitions.
+
+Require Import FMapWeakList  RelationClasses Relation_Definitions Morphisms SetoidClass.
+
+Require Import Coq.Structures.DecidableTypeEx.
+
+Module Type AbstractStore (VT : ValType).
+  Parameter t : Type.
+  Parameter tS : Setoid t.
+  Parameter update : varS ~> VT.valS ~~> tS ~~> tS.
+  Notation "store [ var ↦ val ]s " := (update @ var @ val @ store) (at level 11).
+End AbstractStore.
+
