QAL/Concrete/Expr.v
@@ -1,4 +1,4 @@
-Require Import Tactics Algebra.Utils SetoidUtils Algebra.SetoidCat Algebra.Monad Algebra.SetoidCat.ListUtils Algebra.SetoidCat.PairUtils Algebra.SetoidCat.MaybeUtils Algebra.Monad.Maybe Algebra.Functor Algebra.Applicative Definitions Algebra.Functor.Monad Algebra.Applicative.Monad Algebra.Traversable.List QAL.Store QAL.Heap.
+Require Import Tactics Algebra.Utils SetoidUtils Algebra.SetoidCat Algebra.Monad Algebra.SetoidCat.ListUtils Algebra.SetoidCat.PairUtils Algebra.SetoidCat.MaybeUtils Algebra.Monad.Maybe Algebra.Functor Algebra.Applicative Algebra.Functor.Monad Algebra.Applicative.Monad Algebra.Traversable.List QAL.Concrete.Store QAL.Concrete.Heap QAL.Definitions QAL.Concrete.Definitions.
 
 Require Import FMapWeakList Coq.Lists.List RelationClasses Relation_Definitions Morphisms SetoidClass.
 
